uiop for BetreeBlockCacheSystem and refinement

disk-betree/BetreeBlockCache.dfy
@@ -22,6 +22,7 @@ module BetreeBlockCache {
 
   type DiskOp = BC.DiskOp
   type Op = BC.Op
+  type UIOp = DB.UIOp
 
   predicate Init(k: Constants, s: Variables) {
     BC.Init(k, s)
@@ -35,16 +36,18 @@ module BetreeBlockCache {
     | BetreeMoveStep(betreeStep: BetreeStep)
     | BlockCacheMoveStep(blockCacheStep: BC.Step)
 
-  predicate BetreeMove(k: Constants, s: Variables, s': Variables, dop: DiskOp, betreeStep: BetreeStep)
+  predicate BetreeMove(k: Constants, s: Variables, s': Variables, uiop: UIOp, dop: DiskOp, betreeStep: BetreeStep)
   {
     && dop.NoDiskOp?
     && s.Ready?
     && ValidBetreeStep(betreeStep)
     && BC.Reads(k, s, BetreeStepReads(betreeStep))
     && BC.OpTransaction(k, s, s', BetreeStepOps(betreeStep))
+    && BetreeStepUI(betreeStep, uiop)
   }
 
-  predicate BlockCacheMove(k: Constants, s: Variables, s': Variables, dop: DiskOp, step: BC.Step) {
+  predicate BlockCacheMove(k: Constants, s: Variables, s': Variables, uiop: UIOp, dop: DiskOp, step: BC.Step) {
+    && uiop.NoOp?
     && (
       || step.WriteBackStep?
       || step.WriteBackSuperblockStep?
@@ -56,15 +59,15 @@ module BetreeBlockCache {
     && BC.NextStep(k, s, s', dop, step)
   }
 
-  predicate NextStep(k: Constants, s: Variables, s': Variables, dop: DiskOp, step: Step) {
+  predicate NextStep(k: Constants, s: Variables, s': Variables, uiop: UIOp, dop: DiskOp, step: Step) {
     match step {
-      case BetreeMoveStep(step) => BetreeMove(k, s, s', dop, step)
-      case BlockCacheMoveStep(step) => BlockCacheMove(k, s, s', dop, step)
+      case BetreeMoveStep(step) => BetreeMove(k, s, s', uiop, dop, step)
+      case BlockCacheMoveStep(step) => BlockCacheMove(k, s, s', uiop, dop, step)
     }
   }
 
-  predicate Next(k: Constants, s: Variables, s': Variables, dop: DiskOp) {
-    exists step: Step :: NextStep(k, s, s', dop, step)
+  predicate Next(k: Constants, s: Variables, s': Variables, uiop: UIOp, dop: DiskOp) {
+    exists step: Step :: NextStep(k, s, s', uiop, dop, step)
   }
 
   lemma InitImpliesInv(k: Constants, s: Variables)
@@ -76,40 +79,40 @@ module BetreeBlockCache {
 
   function BIStepsToOps(step: seq<BI.Step>) : seq<Op>
 
-  lemma BetreeMoveStepPreservesInv(k: Constants, s: Variables, s': Variables, dop: DiskOp, betreeStep: BetreeStep)
+  lemma BetreeMoveStepPreservesInv(k: Constants, s: Variables, s': Variables, uiop: UIOp, dop: DiskOp, betreeStep: BetreeStep)
   requires Inv(k, s)
-  requires BetreeMove(k, s, s', dop, betreeStep)
+  requires BetreeMove(k, s, s', uiop, dop, betreeStep)
   ensures Inv(k, s')
   {
     var ops :| BC.OpTransaction(k, s, s', ops);
     BC.TransactionStepPreservesInvariant(k, s, s', D.NoDiskOp, ops);
   }
 
-  lemma BlockCacheMoveStepPreservesInv(k: Constants, s: Variables, s': Variables, dop: DiskOp, step: BC.Step)
+  lemma BlockCacheMoveStepPreservesInv(k: Constants, s: Variables, s': Variables, uiop: UIOp, dop: DiskOp, step: BC.Step)
   requires Inv(k, s)
-  requires BlockCacheMove(k, s, s', dop, step)
+  requires BlockCacheMove(k, s, s', uiop, dop, step)
   ensures Inv(k, s')
   {
     BC.NextStepPreservesInv(k, s, s', dop, step);
   }
 
-  lemma NextStepPreservesInv(k: Constants, s: Variables, s': Variables, dop: DiskOp, step: Step)
+  lemma NextStepPreservesInv(k: Constants, s: Variables, s': Variables, uiop: UIOp, dop: DiskOp, step: Step)
   requires Inv(k, s)
-  requires NextStep(k, s, s', dop, step)
+  requires NextStep(k, s, s', uiop, dop, step)
   ensures Inv(k, s')
   {
     match step {
-      case BetreeMoveStep(step) => BetreeMoveStepPreservesInv(k, s, s', dop, step);
-      case BlockCacheMoveStep(step) => BlockCacheMoveStepPreservesInv(k, s, s', dop, step);
+      case BetreeMoveStep(step) => BetreeMoveStepPreservesInv(k, s, s', uiop, dop, step);
+      case BlockCacheMoveStep(step) => BlockCacheMoveStepPreservesInv(k, s, s', uiop, dop, step);
     }
   }
 
-  lemma NextPreservesInv(k: Constants, s: Variables, s': Variables, dop: DiskOp)
+  lemma NextPreservesInv(k: Constants, s: Variables, s': Variables, uiop: UIOp, dop: DiskOp)
   requires Inv(k, s)
-  requires Next(k, s, s', dop)
+  requires Next(k, s, s', uiop, dop)
   ensures Inv(k, s')
   {
-    var step: Step :| NextStep(k, s, s', dop, step);
-    NextStepPreservesInv(k, s, s', dop, step);
+    var step: Step :| NextStep(k, s, s', uiop, dop, step);
+    NextStepPreservesInv(k, s, s', uiop, dop, step);
   }
 }
